% !TeX root = ../cosmology_main.tex
%=========================================================
%=========================================================
\chapter{Cosmic Microwave Background}\label{ch:cmb}
%========================================================
%=========================================================



%--------------------------------------------------------
%=========================================================
\section{Geodesic \& Boltzmann Equations for photons}
%=========================================================
%------------------------------------------------------------

We specialize the newtonian-gauge geodesic equations \eqref{eq:geodesic_equation_covariant_momentum_newtonian}-\eqref{eq:geodesic_equation_physical_momentum_newtonian} and the Boltzmann equation \eqref{eq:Boltzmann_LHS_exact_newton_gauge} to the case of photons $p=E$. 
We have 
\begin{align}\label{eq:geodesic_equations_photon_newtonian}
\begin{aligned}
    \frac{d P^0}{d\lambda}
    &= -\frac{E^2}{a^2}\left(\mathcal{H}(1-2\psi)+\dot\psi\right)-2\frac{Ep}{a^2}\hat{p}^j\partial_j\psi-\frac{p^2}{a^2}\left(\mathcal{H}(1-2\psi)+\dot\phi\right),
    \\
    \frac{dP^k}{d\lambda}&=-\frac{E^2}{a^2}\partial_k\psi-\frac{Ep}{a^2}\hat{p}^k\,2\left(\mathcal{H}(1-\psi+\phi)-\dot\phi\right)-\frac{p^2}{a^2}\left(\partial_k\phi-2\hat{p}^k\hat{p}^j\partial_j\phi\right).
    \\
    \frac{d E}{d\ct}&=-\frac{p^2}{E}(\mathcal{H}-\dot\phi)-\hat{p}^j\partial_j\psi,
    \\
    \frac{d p}{d\ct}&=-p(\mathcal{H}-\dot\phi)-\frac{E}{p}\hat{p}^j\partial_j\psi,
    \\
    \frac{d\hat{p}^i}{d\ct}&=\big(\hat{p}^i\hat{p}^j-\delta^{ij}\big)\left(\frac{E}{p}\partial_j\psi+\frac{p}{E}\partial_j\phi\right).
\end{aligned}
\end{align}
Similarly, the Boltzmann equation for photons becomes
{\small
\begin{align}\label{eq:Boltzmann_LHS_exact_newton_gauge_photon}
\begin{aligned}
    \frac{d f}{d \lambda}
    %
    &=
    %
    P^{0}\left[\frac{\partial f}{\partial \tau}+\frac{\partial f}{\partial x^{i}} \frac{P^{i}}{P^{0}}+\frac{\partial f}{\partial E} \frac{1}{P^{0}} \frac{d E}{d \lambda}+\frac{\partial f}{\partial \hat{p}^{i}} \frac{1}{P^{0}} \frac{d \hat{p}^{i}}{d \lambda}\right]
    %
    \\&=
    %
    \frac{E}{a}\!\left[\frac{\partial f}{\partial \ct}(1-\psi)
    \!+\!\left(\hat{p}^j\partial_jf\right) \frac{p}{E}(1\!+\!\phi)
    -\frac{\partial f}{\partial E}\frac{p^2}{E}\left(\mathcal{H}(1\!-\!\psi)-\dot\phi\right)
    -\frac{\partial f}{\partial \bar{p}^j}\partial_j\psi \,E
    \!+\!\left(\frac{\partial f}{\partial p} \hat{p}^j-\frac{\partial f}{\partial \bar{p}^j}\right)\partial_j\phi\,\frac{p^2}{E}\right].
\end{aligned}
\end{align}}

Photons retain local equilibrium with a blackbody distribution at all time\todotag{Discuss}, simply with a time and momentum dependent temperature, 
{\small
\begin{equation}\label{eq:local_temp_photons}
    f(\ct, x^i, E, \hat{p}^i) = \frac{1}{\exp\left(\frac{E}{T(\ct, x^i)}\right) - 1}, \quad T=\bar{T}(\tau)(1+\Theta(\tau, x^i, p, \hat{p}^i))=\bar{T}+\delta T.
\end{equation}}
In fact, the argument below hold more generally assuming the distribution is some function $f(E/T)$ of the ratio $E/T$ to some \emph{local} temperature.
At late times collisions with baryons are essentially low-energy elastic Compton scatterings, which do not change the momenetum of photons but only the direction.
To good approximation we can assume $\Theta=\Theta(\tau, x^i, \hat{p}^i)$, i.e. the temperature perturbation is independent of the photon energy.
We can then expand the Boltzmann distribution and its derivatives as\todotag{Ceck}
\begin{align}
\begin{aligned}
    f= \bar{f}+\frac{\partial f}{\partial T}\delta T = \bar{f}-\frac{\partial \bar{f}}{\partial E}\frac{E}{T}\Theta,\\
    \frac{\partial f}{\partial E}=\frac{\partial \bar{f}}{\partial E}-\frac{\partial^2 \bar{f}}{\partial E^2}\frac{E}{T}\Theta-\frac{\partial \bar{f}}{\partial E}\frac{1}{T}\Theta,\\
    \frac{\partial f}{\partial p}=\frac{\partial \bar{f}}{\partial p}-\frac{\partial^2 \bar{f}}{\partial p^2}\frac{p}{T}\Theta-\frac{\partial \bar{f}}{\partial p}\frac{1}{T}\Theta,\\
    \frac{\partial f}{\partial \hat{p}^i}=-\frac{\partial^2 \bar{f}}{\partial p^2}\frac{p}{T}\Theta\hat{p}^i-\frac{\partial \bar{f}}{\partial p}\frac{1}{T}\Theta\hat{p}^i-\frac{\partial \bar{f}}{\partial p}\frac{1}{T}\frac{\partial \Theta}{\partial \hat{p}^i}.
\end{aligned}
\end{align}








%--------------------------------------------------------
%=========================================================
\section{CMB Lensing}
%=========================================================
%------------------------------------------------------------